Switch State_i register files from function to tree for faster normalization

tools/Vale/src/emit_common_quick_code.fs
@@ -245,6 +245,13 @@ let build_qcode (env:env) (loc:loc) (p:proc_decl) (ss:stmt list):decls =
 let build_proc_body (env:env) (loc:loc) (p:proc_decl) (code:exp) (ens:exp):stmt list =
   let makeArg (x, t, storage, io, attrs) = EVar x
   let args = List.map makeArg p.pargs in
+  // let va_old = expand_state va_old in
+  let expand_arg (x, t, _, _, a) =
+    if attrs_get_bool (Reserved "expand_arg") false a then
+      [SAssign ([(x, None)], EApply (Id "expand_state", [EVar x]))]
+    else []
+    in
+  let expansions = List.collect expand_arg p.pargs in
   // let (sM, fM, g) = wpSound_X code (qCodes_X ARGS) s0 (fun s0 sM gs -> let (g1, ..., gn) = g in ENS) in
   // let (g1, ..., gn) = g in
   let s0 = Reserved "s0" in
@@ -266,4 +273,4 @@ let build_proc_body (env:env) (loc:loc) (p:proc_decl) (code:exp) (ens:exp):stmt 
     | [] -> []
     | _ -> [SAssign (gAssigns, EVar g)]
     in
-  [sWpSound] @ sAssignGs
+  expansions @ [sWpSound] @ sAssignGs
