src/arch/x64/X64.Vale.Xmms_i.fst
@@ -2,7 +2,7 @@ module X64.Vale.Xmms_i
 open X64.Machine_s
 open FStar.FunctionalExtensionality
 
-let equal xmms1 xmms2 = feq xmms1 xmms2
-let lemma_equal_intro xmms1 xmms2 = ()
+let equal xmms1 xmms2 = xmms1 == xmms2
+let lemma_equal_intro xmms1 xmms2 = Map16_i.lemma_equal xmms1 xmms2
 let lemma_equal_elim xmms1 xmms2 = ()
 
