src/arch/x64/X64.Vale.Xmms_i.fsti
@@ -4,12 +4,12 @@ module X64.Vale.Xmms_i
 open X64.Machine_s
 unfold let quad32 = Types_s.quad32
 
-type t = xmm -> quad32
+type t = Map16_i.map quad32
 
 val equal : xmms1:t -> xmms2:t -> Type0
 
 val lemma_equal_intro : xmms1:t -> xmms2:t -> Lemma
-  (requires forall x. xmms1 x == xmms2 x)
+  (requires forall (x:xmm). Map16_i.sel xmms1 x == Map16_i.sel xmms2 x)
   (ensures equal xmms1 xmms2)
   [SMTPat (equal xmms1 xmms2)]
 
